%% Appendix-Notes.tex
%% Mac Radigan

\section{Appendix D: Notes}
\label{sec:appendix_notes}
\subsection{Y-Combiner}

% \begin{displayquote}
% Tiger got to hunt, bird got to fly;
% \newline
% Man got to sit and wonder 'why, why, why?'
% \newline
% Tiger got to sleep, bird got to land;
% \newline
% Man got to tell himself he understand.
% \newline
% -Kurt Vonnegut, Cat's Cradle
% \end{displayquote}
% 
% \newline
% \newline
% 
% \begin{displayquote}
% Tiger got to hunt,
% \newline
% Bird got to fly;
% \newline
% Lisper got to sit and wonder, (Y (Y Y))?
% \newline
% \newline
% Tiger got to sleep,
% \newline
% Bird got to land;
% \newline
% Lisper got to tell himself he understand.
% \newline
% - Kurt Vonnegut, modified by Darius Bacon
% \end{displayquote}

Curry's Y-Combiner \cite{WikiY} is defined as:

\begin{equation}
\mathbf{Y} = 
\lambda f . 
\left( \lambda x . f \left( x x \right) \right)
\left( \lambda x . f \left( x x \right) \right)
\label{eq:y_combiner}
\end{equation}

When applied to a function $g$, the expansion follows \cite{WikiY}

\begin{equation}
\begin{aligned}
\mathbf{Y}g 
& = \left( \lambda f .  \left( \lambda x . f \left( x x \right) \right) \left( \lambda x . f \left( x x \right) \right) \right) g \\
& = \left( \lambda x . g \left( x x \right) \right) \left( \lambda x . g \left( x x \right) \\
& = g \left( \left( \lambda x . g \left( x x \right) \right) \left( \lambda x . g \left( x x \right) \right) \\
& = g \left( \mathbf{Y} g \right)
\end{aligned}
\label{eq:y_combiner}
\end{equation}



%% *EOF*
